concurrency/lifting_safety.v
@@ -1,0 +1,372 @@
+From mathcomp.ssreflect Require Import ssreflect seq ssrbool ssrnat.
+
+Require Import compcert.common.Memory.
+Require Import compcert.common.Globalenvs.
+
+(* The concurrent machinery*)
+Require Import concurrency.concurrent_machine.
+Require Import concurrency.dry_machine. Import Concur.
+Require Import concurrency.scheduler.
+
+Require Import concurrency.lifting.
+
+(* We lift to a whole-program simulation on the dry concurrency machine *)
+Require Import sepcomp.wholeprog_simulations. Import Wholeprog_sim.
+
+Require Import sepcomp.event_semantics.
+
+(** The X86 DryConc Machine*)
+Require Import concurrency.dry_context.
+
+(** The Clight DryConc Machine*)
+Require Import concurrency.DryMachineSource.
+
+Require Import concurrency.machine_simulation. Import machine_simulation.
+
+
+Module lifting_safety (SEMT: Semantics) (Machine: MachinesSig with Module SEM := SEMT).
+  Module lftng:= lifting SEMT Machine. Import lftng.
+  Module foo:= Machine.
+
+  Definition match_st gT gS main p sch:=
+    Machine_sim.match_state
+      _ _ _ _ _ _ _ _
+      (concur_sim gT gS main p sch).
+
+  Definition running_thread gT gS main p sch:=
+    Machine_sim.thread_running
+      _ _ _ _ _ _ _ _
+      (concur_sim gT gS main p sch).
+
+  Definition halt_axiom gT gS main p sch:=
+    Machine_sim.thread_halted
+      _ _ _ _ _ _ _ _
+      (concur_sim gT gS main p sch).
+
+(*  THE_DRY_MACHINE_SOURCE.dmachine_state
+    Machine.DryConc.MachState
+ *)
+  (* This axiom comes from the new simulation*)
+  (*Axiom blah: forall  Tg Sg main p U,
+    forall cd j Sm Tm Sds Tds,
+      (match_st Tg Sg main p U) cd j Sds Sm Tds Tm ->
+      forall sch,
+        THE_DRY_MACHINE_SOURCE.DryMachine.valid  (sch, snd (fst Sds), snd Sds) <->
+        Machine.DryConc.valid (sch, snd (fst Tds), snd Tds). *)
+
+      Axiom halted_trace: forall U tr tr' st,
+          THE_DRY_MACHINE_SOURCE.DryMachine.halted (U, tr, st) ->
+          THE_DRY_MACHINE_SOURCE.DryMachine.halted (U, tr', st).
+      Axiom halted_trace': forall U tr tr' st,
+          Machine.DryConc.halted (U, tr, st) ->
+          Machine.DryConc.halted (U, tr', st).
+
+      
+      
+  Lemma safety_preservation': forall main p U Sg Tg tr Sds Sm Tds Tm
+      (MATCH: exists cd j, (match_st Tg Sg main p U) cd j Sds Sm Tds Tm),
+      (forall sch, THE_DRY_MACHINE_SOURCE.DryMachine.valid (sch, tr, Sds) ->
+              THE_DRY_MACHINE_SOURCE.DryMachine.explicit_safety Sg sch Sds Sm) ->
+      (forall sch, Machine.DryConc.valid (sch, tr, Tds) ->
+              Machine.DryConc.explicit_safety Tg sch Tds Tm).
+  Proof.
+    move => main p U Sg Tg.
+    cofix.
+    intros.
+    assert (H':=H).
+    specialize (H sch).
+    move: MATCH => [] cd [] j MATCH.
+    assert (equivalid: forall  Tg Sg main p U,
+               forall cd j Sm Tm tr Sds Tds,
+                 (match_st Tg Sg main p U) cd j Sds Sm Tds Tm ->
+                 forall sch,
+                   THE_DRY_MACHINE_SOURCE.DryMachine.valid (sch, tr, Sds)  <->
+                   Machine.DryConc.valid (sch, tr, Tds) ).
+    { 
+      rewrite /THE_DRY_MACHINE_SOURCE.DryMachine.valid
+              /THE_DRY_MACHINE_SOURCE.SCH.schedPeek
+              /Machine.DryConc.valid
+              /mySchedule.schedPeek /=.
+      move => ? ? ? ? ? ? ? ? ? ? ? Tds' /(running_thread) /= -> U''.
+      
+      destruct (Machine.DryConc.running_thread (Tds')); intuition.
+    }
+    move: (MATCH) => /equivalid /= AA.
+    move: (AA tr sch) => [A B].
+    assert (HH:THE_DRY_MACHINE_SOURCE.DryMachine.valid (sch, tr, Sds)).
+    { apply: B.
+      apply: H0. }
+    apply H in HH.
+    move: MATCH.
+    inversion HH.
+    (*Halted case*)
+    - {
+      simpl in *; subst.
+      econstructor.
+      move: MATCH H1 => /halt_axiom /= HHH /(halted_trace _ nil nil Sds) AAA.
+      destruct (THE_DRY_MACHINE_SOURCE.DryMachine.halted (sch, nil ,Sds)) eqn:BBB; try solve [inversion AAA].
+      move: BBB=> /HHH [] j' [] v2 [] inv Halt.
+      rewrite Halt=> //.
+      rewrite BBB in AAA; inversion AAA.
+      }
+      (*Internal Step case*)
+    - { simpl in *; subst.
+        assert (my_core_diagram:= Machine_sim.thread_diagram
+                           _ _ _ _ _ _ _ _
+                           (concur_sim Tg Sg main p U)).
+        simpl in my_core_diagram.
+        intros MATCH.
+        eapply my_core_diagram with (st1':= (st'))(m1':=m') in MATCH; eauto.
+        clear my_core_diagram.
+        move: MATCH => [] st2' [] m2' [] cd' [] mu' [] MATCH' [step_plus | [] [] n stepN data_step ].
+        (*Internal step Plus*)
+        - inversion step_plus.
+          move: H3=> [] st2'' [] m2'' [] t_step t_stepN.
+          eapply (Machine.DryConc.internal_safety Tg sch (Tds) Tm).
+          + apply: t_step.
+          + specialize (safety_preservation' nil (st') m' st2' m2').
+            cut (exists cd j, match_st Tg Sg main p U cd j (st') m' st2' m2').
+            { move /safety_preservation' => condition.
+              move: H2 => /condition.
+              rewrite / Machine.DryConc.new_valid /Machine.DryConc.mk_ostate /=.
+              clear -t_stepN.
+              rename Tg into ge.
+              rename st2'' into st2.
+              rename m2'' into m2.
+              rename x into n.
+              move=> condiction.
+              move: st2 m2 sch t_stepN.
+              (*Make this a separated lemma*)
+              induction n.
+              - intros.
+                inversion t_stepN.
+                apply: condiction.
+                subst; move: H; rewrite /Machine.DryConc.valid /= //.
+              - intros.
+                assert (DeterminismN: forall n,
+                           machine_semantics_lemmas.thread_stepN
+                             (Machine.DryConc.new_MachineSemantics U p) ge n sch st2
+                             m2 st2' m2' ->
+                           forall U', Machine.DryConc.valid (U', [::], st2) ->
+                                 machine_semantics_lemmas.thread_stepN
+                                   (Machine.DryConc.new_MachineSemantics U p) ge n U' st2
+                                   m2 st2' m2'
+                       ).
+              admit. (*This is true by determinism. *)
+              eapply DeterminismN in t_stepN; eauto.
+              inversion t_stepN. 
+              move: H0 => /= [] m_ [] istep stepN.
+              eapply Machine.DryConc.internal_safety; eauto.
+          }
+            { exists cd', mu'=> //. }
+        (*Step star with the data step*)
+        - destruct n.
+         (* the zero case *)
+          + inversion stepN; subst.
+            {
+            eapply safety_preservation'.
+            admit.
+            admit.
+            admit.
+            }
+            
+          (*Same as the step_N case: *)
+          + {
+              admit.
+            }
+      }
+    (*External Step case*)
+    - { assert (my_machine_diagram:= Machine_sim.machine_diagram
+                           _ _ _ _ _ _ _ _
+                           (concur_sim Tg Sg main p U)).
+        simpl in my_machine_diagram.
+        intros MATCH.
+        eapply my_machine_diagram with (st1':= (st'))(m1':=m') in MATCH; eauto.
+        clear my_machine_diagram.
+        move: MATCH => [] st2' [] m2' [] cd' [] mu' [] MATCH' step.
+        eapply (Machine.DryConc.external_safety); eauto.
+      }
+  Admitted.
+
+
+  
+        
+        
+        
+        
+            
+            
+            
+            
+            
+         
+         
+            
+              
+
+              inversion t_stepN. clear t_stepN.
+              move: H0 => [] m_ [] t_step t_stepN'.
+              apply: Machine.DryConc.internal_safety => //.
+              move: (t_step) => /=.
+              cut ( (fst st2 = nil) /\ (fst x = nil));
+                [ clear t_step; move=> [] -> -> t_step | (inversion t_step; split; reflexivity)].
+              
+              
+              
+            eapply t_step.
+              
+              
+              eapply IHn in t_stepN'.
+              
+            eapply condition in H2.
+          eapply safety_preservation' in MATCH'.
+          clear - t_stepN safety_preservation'.
+           
+
+        
+        
+        move: H3 => [] st2' [] m2' [] cd' [] mu' [] MATCH' [ [] n steps' | [] steps' cordr  ].
+        {
+          
+          assert (SFT: forall sch,
+                     Machine.DryConc.valid (sch, snd (fst st2'), snd st2') -> 
+                     Machine.DryConc.safe_new_step Tg (sch, snd (fst st2'), snd st2')  m2').
+          { eapply safety_preservation.
+            * exists cd', mu' => //.
+                unfold match_st.
+                eapply MATCH'.
+              * intros. rewrite /THE_DRY_MACHINE_SOURCE.DryMachine.mk_ostate
+                                /THE_DRY_MACHINE_SOURCE.DryMachine.safe_new_step
+                                /THE_DRY_MACHINE_SOURCE.DryMachine.mk_nstate /=.
+                destruct st' as [[x y] z]=> /=.
+                eapply H2 => //. }
+          assert (VAL:Machine.DryConc.valid (sch, snd (fst Tds), snd Tds)).
+
+
+
+          
+  
+  Lemma safety_preservation: forall main p U Sg Tg Sds Sm Tds Tm
+      (MATCH: exists cd j, (match_st Tg Sg main p U) cd j Sds Sm Tds Tm),
+      (forall sch, THE_DRY_MACHINE_SOURCE.DryMachine.valid (sch, fst Sds, snd Sds) ->
+              THE_DRY_MACHINE_SOURCE.DryMachine.safe_new_step Sg (sch, fst Sds, snd Sds) Sm) ->
+      (forall sch, Machine.DryConc.valid (sch, fst Tds, snd Tds) ->
+  Machine.DryConc.safe_new_step Tg (sch, fst Tds, snd Tds) Tm).
+  Proof.
+    move => main p U Sg Tg.
+    assert (ax:= blah Tg Sg main p U).
+    cofix.
+    intros.
+    assert (H':=H).
+    specialize (H sch).
+    move: MATCH => [] cd [] j MATCH.
+    move: (MATCH) => /blah /= AA.
+    move: (AA sch) => [A B].
+    assert (HH:THE_DRY_MACHINE_SOURCE.DryMachine.new_valid
+             (THE_DRY_MACHINE_SOURCE.DryMachine.mk_nstate Sds Sm) sch).
+    { rewrite /THE_DRY_MACHINE_SOURCE.DryMachine.new_valid
+              /THE_DRY_MACHINE_SOURCE.DryMachine.mk_ostate
+              /THE_DRY_MACHINE_SOURCE.DryMachine.mk_nstate /=.
+      destruct Sds as [[a b] c] => /=; simpl in B.
+      apply: B.
+      apply: H0. }
+    apply H in HH.
+    inversion HH.
+    inversion H1.
+    (*Halted case*)
+    - {
+      destruct Sds as [[a b] c]; simpl in *; subst.
+      econstructor.
+      + (*Notice I Don't use core_halted! might remove it from simulation!!*)
+        econstructor.
+        move: H9;
+          rewrite /THE_DRY_MACHINE_SOURCE.DryMachine.halted
+                  /Machine.DryConc.halted /= //.
+      + rewrite /Machine.DryConc.mk_nstate => U''/= VAL.
+        unfold Machine.DryConc.safe_new_step,
+        Machine.DryConc.mk_nstate in safety_preservation.
+        simpl in safety_preservation.
+        apply: safety_preservation => //.
+        * exists cd, j; apply: MATCH.
+        * move =>  sch.
+          move: H2. rewrite /THE_DRY_MACHINE_SOURCE.DryMachine.safe_new_step
+                            /THE_DRY_MACHINE_SOURCE.DryMachine.mk_nstate /=.
+          destruct st' as [[a' b' ] c']=> /= HH2.
+          apply: HH2.
+      }
+      (*Step case*)
+    - { assert (my_core_diagram:= core_diagram
+                           _ _ _ _ _ _ _ _
+                           (concur_sim Tg Sg main p U)).
+        eapply my_core_diagram with (cd:=cd)(mu:=j)(st2:=(sch, snd (fst Tds), snd Tds))(m2:=Tm) in H3 . clear my_core_diagram.
+        move: H3 => [] st2' [] m2' [] cd' [] mu' [] MATCH' [ [] n steps' | [] steps' cordr  ].
+        {
+          
+          assert (SFT: forall sch,
+                     Machine.DryConc.valid (sch, snd (fst st2'), snd st2') -> 
+                     Machine.DryConc.safe_new_step Tg (sch, snd (fst st2'), snd st2')  m2').
+          { eapply safety_preservation.
+            * exists cd', mu' => //.
+                unfold match_st.
+                eapply MATCH'.
+              * intros. rewrite /THE_DRY_MACHINE_SOURCE.DryMachine.mk_ostate
+                                /THE_DRY_MACHINE_SOURCE.DryMachine.safe_new_step
+                                /THE_DRY_MACHINE_SOURCE.DryMachine.mk_nstate /=.
+                destruct st' as [[x y] z]=> /=.
+                eapply H2 => //. }
+          assert (VAL:Machine.DryConc.valid (sch, snd (fst Tds), snd Tds)).
+          
+          
+          { eapply A=>//. 
+          clear H0 MATCH A B AA. (*Tds*)
+          clear H HH H1 H4 H5. (*sch*)
+          clear MATCH'. (*st2'*)
+          move: m2' st2' SFT sch Tm Tds steps'.
+          
+          induction n.
+          - move => m2' st2' SFT sch Tm Tds steps'.
+            inversion steps'. move: H =>[] m2'' [] STEP' nothing. 
+            inversion nothing; subst.
+            econstructor.
+            + instantiate(2:=Machine.DryConc.mk_nstate st2' m2'); instantiate (1:=fst (fst st2')).
+              econstructor 2.
+              move: STEP'.
+              destruct Tds as [[x y ] z];
+                destruct st2' as [[x' y'] z']=> //.
+            + by rewrite /Machine.DryConc.new_valid /Machine.DryConc.mk_nstate.
+              
+          - move => m2' st2' SFT sch Tm Tds steps'.
+            inversion steps'. move: H => [] m2 [] STEP steps''. 
+            simpl in STEP.
+            econstructor.
+            + instantiate (2:= Machine.DryConc.mk_nstate x m2); instantiate (1:= fst (fst x)).
+              econstructor 2.
+              move: STEP; rewrite /Machine.DryConc.mk_nstate /Machine.DryConc.mk_ostate /Machine.DryConc.MachStep /= => STEP.
+              eapply STEP.
+            + move=> U'' VAL.
+              move: (IHn m2 x); clear IHn.
+              destruct x as [[a b ] c].
+              rewrite /Machine.DryConc.safe_new_step
+                      /Machine.DryConc.mk_nstate
+                      /Machine.DryConc.mk_ostate => /= IHn /=.
+              simpl in VAL.
+              specialize (STEPS a m2 (a, b ,c)).
+              simpl in STEPS. simpl in steps''. eapply STEPS in steps''.
+              simpl.
+              
+          
+
+          => STEP'.
+          eapply STEP'.
+        
+        
+        rewrite /Machine.DryConc.safe_new_step
+                /Machine.DryConc.mk_nstate /=.
+        eapply (safety.csft_step _ _) .
+        econstructor 2.
+face        
+        move: my_core_diagram.
+        
+
+        rewrite /corestep /THE_DRY_MACHINE_SOURCE.DryMachine.MachineSemantics.
+        simpl.
